pull PackedStringArrays from branch psa-bucket

lib/Buckets/PackedStringArray.i.dfy
@@ -9,17 +9,32 @@ module PackedStringArray {
   import opened NativePackedInts
   import opened NativeArrays
   import Uint32_Order
+  import opened Sequences
   
-  datatype Psa = Psa(offsets: seq<uint32>, data: seq<byte>)
+  datatype Psa = Psa(offsets: seq<uint32>, data: seq<NativeTypes.byte>)
 
   predicate WF(psa: Psa)
   {
     && |psa.offsets| < 0x1_0000_0000
+    && |psa.data| < 0x1_0000_0000
     && (|psa.offsets| == 0 ==> |psa.data| == 0)
     && (|psa.offsets| > 0 ==> |psa.data| == psa.offsets[|psa.offsets|-1] as int)
     && Uint32_Order.IsSorted(psa.offsets)
   }
 
+  // TODO psa prefix is silly. Clean up.
+  function method psaNumStrings(psa: Psa) : uint64
+    requires |psa.offsets| < Uint64UpperBound()
+  {
+    |psa.offsets| as uint64
+  }
+  
+  function method psaTotalLength(psa: Psa) : uint64
+    requires |psa.data| < Uint64UpperBound()
+  {
+    |psa.data| as uint64
+  }
+  
   function method psaStart(psa: Psa, i: uint64) : (start : uint32)
   requires WF(psa)
   requires 0 <= i as int < |psa.offsets|
@@ -30,6 +45,17 @@ module PackedStringArray {
       psa.offsets[i-1]
   }
 
+  lemma psaStartsLte(psa: Psa, i: uint64, j: uint64)
+  requires WF(psa)
+  requires 0 <= i as int <= j as int < |psa.offsets|
+  ensures psaStart(psa, i) <= psaStart(psa, j)
+  {
+    if i == 0 {
+    } else {
+      Uint32_Order.IsSortedImpliesLte(psa.offsets, i as int - 1, j as int - 1);
+    }
+  }
+    
   function method psaEnd(psa: Psa, i: uint64) : (end : uint32)
   requires WF(psa)
   requires 0 <= i as int < |psa.offsets|
@@ -43,6 +69,17 @@ module PackedStringArray {
     psa.offsets[i]
   }
 
+  lemma psaStartLtePsaEnd(psa: Psa, i: uint64, j: uint64)
+    requires WF(psa)
+    requires 0 <= i as int <= j as int < |psa.offsets|
+    ensures psaStart(psa, i) <= psaEnd(psa, j)
+  {
+    if i == 0 {
+    } else {
+      Uint32_Order.IsSortedImpliesLte(psa.offsets, i as int - 1, j as int);
+    }
+  }
+  
   function method psaElement(psa: Psa, i: uint64) : seq<byte>
   requires WF(psa)
   requires 0 <= i as int < |psa.offsets|
@@ -65,6 +102,14 @@ module PackedStringArray {
     psaSeq(psa, |psa.offsets|)
   }
 
+  function method EmptyPsa() : (result: Psa)
+    ensures WF(result)
+    ensures I(result) == []
+  {
+    assert Uint32_Order.IsSorted([]) by { Uint32_Order.reveal_IsSorted(); }
+    Psa([], [])
+  }
+  
   function SizeOfPsa(psa: Psa) : int {
     4 + 4 * |psa.offsets| + |psa.data|
   }
@@ -102,15 +147,27 @@ module PackedStringArray {
   requires |s| < 0x1_0000_0000_0000_0000
   ensures b == Uint32_Order.IsSorted(s)
   {
-    assume false;
     var i: uint64 := 1;
+    if |s| < 2 {
+      assert Uint32_Order.IsSorted(s) by { Uint32_Order.reveal_IsSorted(); }
+      return true;
+    }
+    if 0 < |s| {
+      assert Uint32_Order.IsSorted(s[..1]) by { Uint32_Order.reveal_IsSorted(); }
+    }
     while i < |s| as uint64
+      invariant i as int <= |s|
+      invariant Uint32_Order.IsSorted(s[..i])
     {
       if s[i-1] > s[i] {
+        assert !Uint32_Order.IsSorted(s) by { Uint32_Order.reveal_IsSorted(); }
         return false;
       }
+      Uint32_Order.SortedAugment(s[..i], s[i]);
+      assert s[..i+1] == s[..i] + [s[i]];
       i := i + 1;
     }
+    assert s == s[..i];
     return true;
   }
 
@@ -260,5 +317,732 @@ module PackedStringArray {
   requires |psa.offsets| > 0
   {
     psaElement(psa, |psa.offsets| as uint64 - 1)
+  }
+
+  function subtractConstant(nums: seq<uint32>, subtrahend: uint32) : (result: seq<uint32>)
+    requires forall i :: 0 <= i < |nums| ==> subtrahend <= nums[i]
+    ensures |result| == |nums|
+    ensures forall i :: 0 <= i < |result| ==> result[i] == nums[i] - subtrahend
+  {
+    if |nums| == 0 then
+      []
+    else
+      subtractConstant(DropLast(nums), subtrahend) + [Last(nums) - subtrahend]
+  }
+
+  method SubtractConstant(nums: seq<uint32>, subtrahend: uint32) returns (result: seq<uint32>)
+    requires forall i :: 0 <= i < |nums| ==> subtrahend <= nums[i]
+    requires |nums| < Uint64UpperBound()
+    ensures result == subtractConstant(nums, subtrahend)
+  {
+    var arr := newArrayFill(|nums| as uint64, 0);
+    var i: uint64 := 0;
+    while i < |nums| as uint64
+      invariant i <= |nums| as uint64
+      invariant forall j :: j < i ==> arr[j] == nums[j] - subtrahend
+    {
+      arr[i] := nums[i] - subtrahend;
+      i := i + 1;
+    }
+    result := arr[..];
+  }
+  
+  function subOffsets(offsets: seq<uint32>, from: uint64, to: uint64) : (result: seq<uint32>)
+    requires Uint32_Order.IsSorted(offsets)
+    requires 0 <= from as int <= to as int <= |offsets|
+  {
+    var suboffsets := offsets[from..to];
+    if from == 0 then
+      suboffsets
+    else
+      assert forall i :: 0 <= i < |suboffsets| ==> offsets[from-1] <= suboffsets[i] by { Uint32_Order.reveal_IsSorted(); }
+      subtractConstant(suboffsets, offsets[from-1])
+  }
+
+  method SubOffsets(offsets: seq<uint32>, from: uint64, to: uint64) returns (result: seq<uint32>)
+    requires Uint32_Order.IsSorted(offsets)
+    requires 0 <= from as int <= to as int <= |offsets|
+    ensures result == subOffsets(offsets, from, to)
+  {
+    var suboffsets := offsets[from..to];
+    if from == 0 {
+      result := suboffsets;
+    } else {
+      assert forall i :: 0 <= i < |suboffsets| ==> offsets[from-1] <= suboffsets[i] by { Uint32_Order.reveal_IsSorted(); }
+      result := SubtractConstant(suboffsets, offsets[from-1]);
+    }
+  }
+  
+  function psaSubSeqInternal(psa: Psa, from: uint64, to: uint64) : (result: Psa)
+    requires WF(psa)
+    requires 0 <= from <= to <= psaNumStrings(psa)
+  {
+    if from == to then
+      EmptyPsa()
+    else 
+      var dataStart := psaStart(psa, from);
+      var dataEnd := psaEnd(psa, to-1);
+      psaStartLtePsaEnd(psa, from, to-1);
+      Psa(subOffsets(psa.offsets, from, to), psa.data[dataStart..dataEnd])
+  }
+
+  lemma WFpsaSubSeq(psa: Psa, from: uint64, to: uint64)
+    requires WF(psa)
+    requires 0 <= from <= to <= psaNumStrings(psa)
+    ensures WF(psaSubSeqInternal(psa, from, to))
+    ensures I(psaSubSeqInternal(psa, from, to)) == I(psa)[from..to]
+  {
+    var subpsa := psaSubSeqInternal(psa, from, to);
+    assert WF(subpsa) by { Uint32_Order.reveal_IsSorted(); }
+    var isubpsa := I(subpsa);
+    var ipsasub := I(psa)[from..to];
+    assert |isubpsa| == |ipsasub|;
+    forall i: uint64 | 0 <= i < |isubpsa| as uint64
+      ensures isubpsa[i] == ipsasub[i]
+    {
+      var dataStart := psaStart(psa, from);
+      var dataEnd := psaEnd(psa, to-1);
+      var subStart := psaStart(subpsa, i);
+      var subEnd := psaEnd(subpsa, i);
+      // WTF.  Why isn't this a simple calc of sequence?  This proof seem very brittle.
+      forall j  | 0 <= j < subEnd - subStart
+        ensures 
+        psa.data[dataStart..dataEnd][subStart..subEnd][j] ==
+        psa.data[dataStart + subStart..dataStart + subEnd][j]
+      {
+        // For example of the brittleness of this proof, converting these asserts to a single calc causes the proof to fail.
+        assert psa.data[dataStart..dataEnd][subStart..subEnd][j] == psa.data[dataStart..dataEnd][subStart + j];
+        assert psa.data[dataStart..dataEnd][subStart..subEnd][j] == psa.data[dataStart + subStart + j];
+        assert psa.data[dataStart + subStart..dataStart + subEnd][j] == psa.data[dataStart + subStart + j];
+      }
+    }
+  }
+
+  function psaSubSeq(psa: Psa, from: uint64, to: uint64) : (result: Psa)
+    requires WF(psa)
+    requires 0 <= from <= to <= psaNumStrings(psa)
+    ensures WF(result)
+    ensures I(result) == I(psa)[from..to]
+  {
+    WFpsaSubSeq(psa, from, to);
+    psaSubSeqInternal(psa, from, to)
+  }
+  
+  method PsaSubSeq(psa: Psa, from: uint64, to: uint64) returns (result: Psa)
+    requires WF(psa)
+    requires 0 <= from <= to <= psaNumStrings(psa)
+    ensures result == psaSubSeq(psa, from, to)
+    ensures WF(psaSubSeq(psa, from, to))
+    ensures I(psaSubSeq(psa, from, to)) == I(psa)[from..to]
+  {
+    if from == to {
+      result := EmptyPsa();
+    } else {
+      var dataStart := psaStart(psa, from);
+      var dataEnd := psaEnd(psa, to-1);
+      psaStartLtePsaEnd(psa, from, to-1);
+      var newoffsets := SubOffsets(psa.offsets, from, to);
+      result := Psa(newoffsets, psa.data[dataStart..dataEnd]);
+      WFpsaSubSeq(psa, from, to);
+    }
+  }
+  
+  method PsaPrefix(psa: Psa, to: uint64) returns (result: Psa)
+    requires WF(psa)
+    requires 0 <= to <= psaNumStrings(psa)
+    ensures WF(result)
+    ensures I(result) == I(psa)[..to]
+  {
+    result := PsaSubSeq(psa, 0, to);
+  }
+  
+  method PsaSuffix(psa: Psa, from: uint64) returns (result: Psa)
+    requires WF(psa)
+    requires 0 <= from <= psaNumStrings(psa)
+    ensures WF(result)
+    ensures I(result) == I(psa)[from..]
+  {
+    result := PsaSubSeq(psa, from, psaNumStrings(psa));
+  }
+  
+  function psaDropLast(psa: Psa) : (result: Psa)
+    requires WF(psa)
+    requires 0 < psaNumStrings(psa)
+    ensures WF(result)
+    ensures I(result) == Sequences.DropLast(I(psa))
+  {
+    WFpsaSubSeq(psa, 0, psaNumStrings(psa)-1);
+    psaSubSeq(psa, 0, psaNumStrings(psa)-1)
+  }
+
+  predicate psaCanAppend(psa: Psa, key: seq<byte>)
+  {
+    && |psa.offsets| < 0x1_0000_0000 - 1
+    && |psa.data| + |key| < 0x1_0000_0000
+  }
+  
+  method PsaCanAppend(psa: Psa, key: seq<byte>) returns (result: bool)
+    requires WF(psa)
+    requires |key| < 0x1_0000_0000
+  {
+    result :=
+      && |psa.offsets| as uint64 < 0x1_0000_0000 - 1
+      && |psa.data| as uint64 + |key| as uint64 < 0x1_0000_0000;
+  }
+  
+  function psaAppend(psa: Psa, key: seq<byte>) : (result: Psa)
+    requires WF(psa)
+    requires psaCanAppend(psa, key)
+    ensures WF(result)
+  {
+    var newdata := psa.data + key;
+    Uint32_Order.SortedAugment(psa.offsets, |newdata| as uint32);
+    Psa(psa.offsets + [|newdata| as uint32], newdata)
+  }
+
+  lemma psaAppendIAppend(psa: Psa, key: seq<byte>)
+    requires WF(psa)
+    requires psaCanAppend(psa, key)
+    ensures I(psaAppend(psa, key)) == I(psa) + [key]
+  {
+    var ipsaa := I(psaAppend(psa, key));
+    var aipsa := I(psa) + [key];
+    assert |ipsaa| == |aipsa|;
+    forall i | 0 <= i < |ipsaa|
+      ensures ipsaa[i] == aipsa[i]
+    {
+    }
+  }
+  
+  lemma psaAppendTotalLength(psa: Psa, key: seq<byte>)
+    requires WF(psa)
+    requires psaCanAppend(psa, key)
+    ensures psaTotalLength(psaAppend(psa, key)) as int == psaTotalLength(psa) as int + |key|
+  {
+  }
+  
+  predicate psaCanAppendSeq(psa: Psa, strs: seq<seq<byte>>)
+    requires WF(psa)
+    decreases |strs|, 0
+  {
+    && |psa.offsets| + |strs| < 0x1_0000_0000
+    && |psa.data| + FlattenLength(FlattenShape(strs)) < 0x1_0000_0000
+  }
+
+  lemma psaCanAppendOne(psa: Psa, str: seq<byte>)
+    requires WF(psa)
+    requires psaCanAppendSeq(psa, [str])
+    ensures psaCanAppend(psa, str)
+  {
+    reveal_FlattenShape();
+    reveal_FlattenLength();
+  }
+  
+  function psaAppendSeq(psa: Psa, strs: seq<seq<byte>>) : (result: Psa)
+    requires WF(psa)
+    requires psaCanAppendSeq(psa, strs)
+    ensures WF(result)
+    ensures I(result) == I(psa) + strs
+    ensures psaTotalLength(result) == psaTotalLength(psa) + FlattenLength(FlattenShape(strs)) as uint64
+    decreases |strs|, 1
+  {
+    if |strs| == 0 then
+      psa
+    else
+      assert strs == DropLast(strs) + [Last(strs)];
+      FlattenShapeAdditive(DropLast(strs), [Last(strs)]);
+      FlattenLengthAdditive(FlattenShape(DropLast(strs)), FlattenShape([Last(strs)]));
+      assert FlattenLength(FlattenShape(DropLast(strs))) <= FlattenLength(FlattenShape(strs));
+      assert |Last(strs)| == FlattenLength(FlattenShape([Last(strs)])) by {
+        reveal_FlattenShape();
+        reveal_FlattenLength();
+      }
+      psaAppendIAppend(psaAppendSeq(psa, DropLast(strs)), Last(strs));
+      psaAppend(psaAppendSeq(psa, DropLast(strs)), Last(strs))
+  }
+
+  lemma psaCanAppendSeqAdditive(psa: Psa, strs1: seq<seq<byte>>, strs2: seq<seq<byte>>)
+    requires WF(psa)
+    ensures psaCanAppendSeq(psa, strs1 + strs2) <==>
+    psaCanAppendSeq(psa, strs1) && psaCanAppendSeq(psaAppendSeq(psa, strs1), strs2)
+  {
+    FlattenShapeAdditive(strs1, strs2);
+    FlattenLengthAdditive(FlattenShape(strs1), FlattenShape(strs2));
+  }
+
+  lemma psaCanAppendSubSeq(psa: Psa, strs: seq<seq<byte>>, from: nat, to: nat)
+    requires WF(psa)
+    requires psaCanAppendSeq(psa, strs)
+    requires from <= to <= |strs|
+    ensures psaCanAppendSeq(psa, strs[from..to])
+  {
+    var strssh := FlattenShape(strs);
+    var strsl := FlattenLength(strssh);
+    
+    var a := strs[..from];
+    var ash := FlattenShape(a);
+    var al := FlattenLength(ash);
+
+    var b := strs[from..to];
+    var bsh := FlattenShape(b);
+    var bl := FlattenLength(bsh);
+    
+    var c := strs[to..];
+    var csh := FlattenShape(c);
+    var cl := FlattenLength(csh);
+
+    assert strs == a + b + c;
+    
+    FlattenShapeAdditive(a + b, c);
+    FlattenShapeAdditive(a, b);
+    //assert strssh == ash + bsh + csh;
+
+    FlattenLengthAdditive(ash + bsh, csh);
+    FlattenLengthAdditive(ash, bsh);
+    //assert strsl == al + bl + cl;
+  }
+  
+  lemma psaAppendSeqAdditive(psa: Psa, strs1: seq<seq<byte>>, strs2: seq<seq<byte>>)
+    requires WF(psa)
+    requires psaCanAppendSeq(psa, strs1 + strs2) ||
+    (psaCanAppendSeq(psa, strs1) && psaCanAppendSeq(psaAppendSeq(psa, strs1), strs2))
+    ensures psaCanAppendSeq(psa, strs1 + strs2) &&
+    (psaCanAppendSeq(psa, strs1) && psaCanAppendSeq(psaAppendSeq(psa, strs1), strs2))
+    ensures psaAppendSeq(psa, strs1 + strs2) == psaAppendSeq(psaAppendSeq(psa, strs1), strs2)
+  {
+    psaCanAppendSeqAdditive(psa, strs1, strs2);
+    if |strs2| == 0 {
+      assert strs1 + strs2 == strs1;
+    } else if |strs2| == 1 {
+    } else {
+      assert strs1 + DropLast(strs2) + [Last(strs2)] == strs1 + strs2;
+      psaCanAppendSeqAdditive(psa, strs1 + DropLast(strs2), [Last(strs2)]);
+    }
+  }
+  
+  function psaFromSeq(strs: seq<seq<byte>>) : (result: Psa)
+    requires psaCanAppendSeq(EmptyPsa(), strs)
+    ensures WF(result)
+    ensures I(result) == strs
+  {
+    psaAppendSeq(EmptyPsa(), strs)
+  }
+
+  lemma psaCanAppendI(psa: Psa)
+    requires WF(psa)
+    ensures psaCanAppendSeq(EmptyPsa(), I(psa))
+    ensures psaAppendSeq(EmptyPsa(), I(psa)) == psa
+    decreases psaNumStrings(psa)
+  {
+    var strs := I(psa);
+    if psaNumStrings(psa) == 0 {
+    } else if psaNumStrings(psa) == 1 {
+      assert psaCanAppendSeq(EmptyPsa(), I(psa)) by {
+        reveal_FlattenShape();
+        reveal_FlattenLength();
+      }
+    } else {
+      var prepsa := psaDropLast(psa);
+      var prestrs := I(prepsa);
+      var last := Last(strs);
+      assert strs == prestrs + [last];
+      psaCanAppendI(prepsa);
+      assert psaCanAppendSeq(EmptyPsa(), strs) by {
+        reveal_FlattenShape();
+        reveal_FlattenLength();
+      }
+    }
+  }
+  
+  method psaSeqTotalLength(strs: seq<seq<byte>>) returns (len: uint64)
+    requires psaCanAppendSeq(EmptyPsa(), strs)
+    ensures len == psaTotalLength(psaAppendSeq(EmptyPsa(), strs))
+  {
+    forall i | 0 <= i <= |strs|
+      ensures psaCanAppendSeq(EmptyPsa(), strs[..i])
+      ensures psaTotalLength(psaAppendSeq(EmptyPsa(), strs[..i])) <= psaTotalLength(psaAppendSeq(EmptyPsa(), strs))
+    {
+        assert strs == strs[..i] + strs[i..];
+        psaAppendSeqAdditive(EmptyPsa(), strs[..i], strs[i..]);
+    }
+
+    var curlen: uint64 := 0;
+    var i: uint64 := 0;
+    while i < |strs| as uint64
+      invariant i as int <= |strs|
+      invariant curlen == psaTotalLength(psaAppendSeq(EmptyPsa(), strs[..i]))
+    {
+      assert strs[..i] == DropLast(strs[..i+1]);
+      psaAppendTotalLength(psaAppendSeq(EmptyPsa(), strs[..i]), strs[i]);
+      curlen := curlen + |strs[i]| as uint64;
+      i := i + 1;
+    }
+    assert strs == strs[..|strs|];
+    len := curlen;
+  }
+  
+  class DynamicPsa {
+    var nstrings: uint64
+    var offsets: array<uint32>
+    var data: array<byte>
+    ghost var Repr: set<object>
+    
+    predicate WF()
+      reads this, this.Repr
+    {
+      && Repr == {this, offsets, data}
+      && offsets.Length < Uint64UpperBound()
+      && data.Length < 0x1_0000_0000 
+      && nstrings as int <= offsets.Length
+      && nstrings < 0x1_0000_0000
+      && (0 < nstrings ==> offsets[nstrings-1] as int < 0x1_0000_0000)
+      && (0 < nstrings ==> offsets[nstrings-1] as int <= data.Length)
+      && Uint32_Order.IsSorted(offsets[..nstrings])
+    }
+
+    function method toPsa() : Psa
+      requires WF()
+      reads this, this.Repr
+    {
+      if 0 == nstrings then
+        EmptyPsa()
+      else 
+        Psa(offsets[..nstrings], data[..offsets[nstrings-1]])
+    }
+
+    method TotalLength() returns (result: uint64)
+      requires WF()
+      ensures result == psaTotalLength(toPsa())
+    {
+      if nstrings == 0 {
+        result := 0;
+      } else {
+        result := offsets[nstrings-1] as uint64;
+      }
+    }
+    
+    predicate canAppend(str: seq<byte>)
+      requires WF()
+      reads this, this.Repr
+    {
+      && psaCanAppend(toPsa(), str)
+      && nstrings < offsets.Length as uint64
+      && psaTotalLength(toPsa()) + |str| as uint64 <= data.Length as uint64
+    }
+    
+    method CanAppendWORealloc(str: seq<byte>) returns (result: bool)
+      requires WF()
+      requires |str| < 0x1_0000_0000
+      ensures result ==> psaCanAppend(toPsa(), str)
+    {
+      var tl := TotalLength();
+      result := 
+        && nstrings < offsets.Length as uint64
+        && nstrings < 0x1_0000_0000 - 1
+        && tl + |str| as uint64 <= data.Length as uint64;
+    }
+    
+    method append(str: seq<byte>)
+      requires WF()
+      requires canAppend(str)
+      ensures WF()
+      ensures toPsa() == psaAppend(old(toPsa()), str)
+      ensures Repr == old(Repr)
+      modifies this.Repr
+    {
+      var start: uint32 := if nstrings == 0 then 0 else offsets[nstrings-1];
+      offsets[nstrings] := start + |str| as uint32;
+      CopySeqIntoArray(str, 0, data, start as uint64, |str| as uint64);
+      nstrings := nstrings + 1;
+      Uint32_Order.reveal_IsSorted();
+    }
+
+    method realloc_offsets(new_offsets_len: uint64)
+      requires WF()
+      requires nstrings <= new_offsets_len
+      ensures WF()
+      ensures toPsa() == old(toPsa())
+      ensures fresh(offsets)
+      ensures offsets.Length == new_offsets_len as int
+      ensures data == old(data)
+      modifies this.Repr
+    {
+      var new_offsets := new uint32[new_offsets_len];
+      CopyArrayIntoDifferentArray(offsets, 0, new_offsets, 0, nstrings);
+      offsets := new_offsets;
+      assert offsets[..nstrings] == old(offsets[..nstrings]);
+      Repr := {this, offsets, data};
+    }
+    
+    method realloc_data(new_data_len: uint64)
+      requires WF()
+      requires new_data_len < 0x1_0000_0000 
+      requires 0 < nstrings ==> offsets[nstrings-1] as uint64 <= new_data_len
+      ensures WF()
+      ensures toPsa() == old(toPsa())
+      ensures offsets == old(offsets)
+      ensures fresh(data)
+      ensures data.Length == new_data_len as int
+      modifies this.Repr
+    {
+      var data_len := if 0 == nstrings then 0 else offsets[nstrings-1];
+      var new_data := new byte[new_data_len];
+      CopyArrayIntoDifferentArray(data, 0, new_data, 0, data_len as uint64);
+      data := new_data;
+      Repr := {this, offsets, data};
+    }
+
+    method realloc_to_accomodate(str: seq<byte>)
+      requires WF()
+      requires psaCanAppend(toPsa(), str)
+      ensures WF()
+      ensures toPsa() == old(toPsa())
+      ensures canAppend(str)
+      ensures fresh(Repr - old(Repr))
+      modifies this.Repr
+    {
+      if nstrings == offsets.Length as uint64 {
+        if 0x8000_0000 <= nstrings {
+          realloc_offsets(0xffff_ffff);
+        } else {
+          realloc_offsets(2*nstrings + 1);
+        }
+      }
+      var data_len: uint32 := if nstrings == 0 then 0 else offsets[nstrings-1];
+      assert data_len as uint64 == psaTotalLength(toPsa());
+      var new_len: uint64 := data_len as uint64 + |str| as uint64;
+      if data.Length as uint64 < new_len {
+        if 0x1_0000_0000 <= 2 * new_len {
+          realloc_data(0xffff_ffff);
+        } else {
+          realloc_data(2*new_len);
+        }
+      }
+    }
+    
+    method Append(str: seq<byte>)
+      requires WF()
+      requires psaCanAppend(toPsa(), str)
+      ensures WF()
+      ensures toPsa() == psaAppend(old(toPsa()), str)
+      ensures fresh(Repr - old(Repr))
+      modifies this.Repr
+    {
+      realloc_to_accomodate(str);
+      append(str);
+    }
+
+    method appendSeq(strs: seq<seq<byte>>)
+      requires WF()
+      requires psaCanAppendSeq(toPsa(), strs)
+      requires nstrings as int + |strs| <= offsets.Length
+      requires psaTotalLength(psaAppendSeq(toPsa(), strs)) as int <= data.Length
+      ensures WF()
+      ensures toPsa() == psaAppendSeq(old(toPsa()), strs)
+      ensures Repr == old(Repr)
+      modifies this, this.Repr
+    {
+      forall i | 0 <= i <= |strs|
+        ensures psaCanAppendSeq(toPsa(), strs[..i])
+        ensures psaTotalLength(psaAppendSeq(toPsa(), strs[..i])) <= psaTotalLength(psaAppendSeq(toPsa(), strs))
+      {
+        assert strs == strs[..i] + strs[i..];
+        psaAppendSeqAdditive(toPsa(), strs[..i], strs[i..]);
+      }
+      
+      var i: uint64 := 0;
+      while i < |strs| as uint64
+        invariant i as int <= |strs|
+        invariant WF()
+        invariant toPsa() == psaAppendSeq(old(toPsa()), strs[..i])
+        invariant Repr == old(Repr)
+      {
+        assert strs[..i+1] == strs[..i] + [strs[i]];
+        append(strs[i]);
+        i := i + 1;
+      }
+      assert strs[..|strs|] == strs;
+    }
+    
+    method realloc_to_accomodate_seq(strs: seq<seq<byte>>)
+      requires WF()
+      requires psaCanAppendSeq(toPsa(), strs)
+      ensures WF()
+      ensures toPsa() == old(toPsa())
+      ensures nstrings as int + |strs| <= offsets.Length
+      ensures psaTotalLength(psaAppendSeq(toPsa(), strs)) as int <= data.Length
+      ensures fresh(Repr - old(Repr))
+      modifies this.Repr
+    {
+      forall i | 0 <= i <= |strs|
+        ensures psaCanAppendSeq(toPsa(), strs[..i])
+        ensures psaTotalLength(psaAppendSeq(toPsa(), strs[..i])) <= psaTotalLength(psaAppendSeq(toPsa(), strs))
+      {
+        assert strs == strs[..i] + strs[i..];
+        psaAppendSeqAdditive(toPsa(), strs[..i], strs[i..]);
+      }
+      
+      if offsets.Length as uint64 < nstrings as uint64 + |strs| as uint64 {
+        realloc_offsets(nstrings as uint64 + |strs| as uint64);
+      }
+
+      var total_len: uint64 := if nstrings == 0 then 0 else offsets[nstrings-1] as uint64;
+      var i: uint64 := 0;
+      while i < |strs| as uint64
+        invariant i as int <= |strs|
+        invariant  total_len as int == psaTotalLength(psaAppendSeq(toPsa(), strs[..i])) as int
+        modifies {}
+      {
+        assert strs[..i] == DropLast(strs[..i+1]);
+        psaAppendTotalLength(psaAppendSeq(toPsa(), strs[..i]), strs[i]);
+        total_len := total_len + |strs[i]| as uint64;
+        i := i + 1;
+      }
+      assert strs == strs[..|strs|];
+      if data.Length as uint64 < total_len {
+        realloc_data(total_len);
+      }
+    }
+    
+    method AppendSeq(strs: seq<seq<byte>>)
+      requires WF()
+      requires psaCanAppendSeq(toPsa(), strs)
+      ensures WF()
+      ensures toPsa() == psaAppendSeq(old(toPsa()), strs)
+      ensures fresh(Repr - old(Repr))
+      modifies this, this.Repr
+    {
+      realloc_to_accomodate_seq(strs);
+      ghost var new_Repr := Repr;
+      ghost var new_offsets := offsets;
+      ghost var new_data := data;
+
+      assert psaTotalLength(psaAppendSeq(toPsa(), strs)) as int <= data.Length;
+      
+      forall i | 0 <= i <= |strs|
+        ensures psaCanAppendSeq(toPsa(), strs[..i])
+      {
+        assert strs == strs[..i] + strs[i..];
+        psaCanAppendSeqAdditive(toPsa(), strs[..i], strs[i..]);
+      }
+
+      forall i | 0 <= i < |strs|
+        ensures psaCanAppend(psaAppendSeq(toPsa(), strs[..i]), strs[i])
+        ensures psaTotalLength(psaAppendSeq(toPsa(), strs[..i])) as int + |strs[i]| <= data.Length
+      {
+        assert strs[..i+1] == strs[..i] + [strs[i]];
+        psaCanAppendSeqAdditive(toPsa(), strs[..i], [strs[i]]);
+        psaCanAppendOne(psaAppendSeq(toPsa(), strs[..i]), strs[i]);
+        assert strs == strs[..i+1] + strs[i+1..];
+        psaAppendSeqAdditive(toPsa(), strs[..i+1], strs[i+1..]);
+      }
+      
+      var i: uint64 := 0;
+      while i < |strs| as uint64
+        invariant i as int <= |strs|
+        invariant WF()
+        invariant toPsa() == psaAppendSeq(old(toPsa()), strs[..i])
+        invariant Repr == new_Repr
+        invariant offsets == new_offsets
+        invariant data == new_data
+      {
+        assert strs[..i+1] == strs[..i] + [strs[i]];
+        append(strs[i]);
+        i := i + 1;
+      }
+      assert strs[..|strs|] == strs;
+    }
+
+    method Prefix(newlen: uint64)
+      requires WF()
+      requires newlen <= nstrings
+      ensures WF()
+      ensures toPsa() == psaSubSeq(old(toPsa()), 0, newlen)
+      ensures offsets == old(offsets)
+      ensures data == old(data)
+      ensures Repr == old(Repr)
+      modifies this
+    {
+      Uint32_Order.SortedSubsequence(offsets[..nstrings], 0, newlen as int);
+      assert offsets[..newlen] == offsets[..nstrings][..newlen];
+      if 0 < newlen {
+        Uint32_Order.IsSortedImpliesLte(offsets[..nstrings], newlen as int - 1, nstrings as int - 1);
+      }
+      nstrings := newlen;
+    }
+    
+    constructor PreSized(num_strings: uint32, total_len: uint32)
+      ensures WF()
+      ensures offsets.Length == num_strings as int
+      ensures data.Length == total_len as int
+      ensures toPsa() == EmptyPsa()
+      ensures fresh(Repr)
+    {
+      nstrings := 0;
+      offsets := new uint32[num_strings];
+      data := new byte[total_len];
+      Repr := {this, offsets, data};
+    }
+
+    constructor FromSeq(strs: seq<seq<byte>>)
+      requires psaCanAppendSeq(EmptyPsa(), strs)
+      ensures WF()
+      ensures offsets.Length == |strs|
+      ensures data.Length == psaTotalLength(psaFromSeq(strs)) as int
+      ensures toPsa() == psaFromSeq(strs)
+      ensures fresh(Repr)
+    {
+      nstrings := 0;
+      offsets := new uint32[|strs| as uint64];
+      var total_len := psaSeqTotalLength(strs);
+      data := new byte[total_len];
+      Repr := {this, offsets, data};
+      new;
+      appendSeq(strs);
+    }
+  }
+
+  method FromSeq(strs: seq<seq<byte>>) returns (psa: Psa)
+    requires psaCanAppendSeq(EmptyPsa(), strs)
+    ensures WF(psa)
+    ensures I(psa) == strs
+  {
+    var dpsa := new DynamicPsa.FromSeq(strs);
+    psa := dpsa.toPsa();
+  }
+
+  method ToSeq(psa: Psa) returns (strs: seq<seq<byte>>)
+    requires WF(psa)
+    ensures strs == I(psa)
+  {
+    var nstrings: uint64 := psaNumStrings(psa);
+    var astrs := new seq<byte>[nstrings];
+
+    var i: uint64 := 0;
+    while i < nstrings
+      invariant i <= nstrings
+      invariant astrs[..i] == psaSeq(psa, i as int)
+    {
+      astrs[i] := psaElement(psa, i);
+      i := i + 1;
+    }
+    strs := astrs[..];
+  }
+  
+  lemma UniqueRepr(psa1: Psa, psa2: Psa)
+    requires WF(psa1)
+    requires WF(psa2)
+    requires I(psa1) == I(psa2)
+    ensures psa1 == psa2
+    decreases |psa1.offsets|
+  {
+    if |psa1.offsets| == 0 {
+    } else {
+      var pre1 := psaDropLast(psa1);
+      var pre2 := psaDropLast(psa2);
+      UniqueRepr(pre1, pre2);
+      var last := Last(I(psa1));
+      assert psa1.data == pre1.data + last;
+    }
   }
 }
